#

$$ f(x) = a - b \tag{1.1} $$
$$ x+2-3*4/6=4/y + x\cdot y $$
$$ 0 \neq 1 \quad x \equiv x \quad 1 = 9 \bmod 2 $$
$$ a*{ij}^{2} + b^3\*{2}=x^{t} + y' + x''\_{12} $$

$$
\sqrt{x} + \sqrt{x^{2}+\sqrt{y}} = \sqrt[3]{k_{i}} - \frac{x}{m}
$$

$$\overline{x+y} \qquad \underline{a+b}$$

$$
\overbrace{1+2+\cdots+n}^{nä¸ª} \qquad \underbrace{a+b+\cdots+z}_{26}
$$

$$\vec{a} + \overrightarrow{AB} + \overleftarrow{DE}$$

$$
\lim_{x \to \infty} x^2_{22} - \int_{1}^{5}x\mathrm{d}x + \sum_{n=1}^{20}
n^{2} = \prod_{j=1}^{3} y_{j} + \lim_{x \to -2} \frac{x-2}{x}
$$

$$
x*{1},x*{2},\ldots,x*{5} \quad x*{1} + x*{2} + \cdots + x*{n}
$$

# Matrix

$$
\begin{pmatrix}
 1 &2  &3  \\
\end{pmatrix}
$$

$$
\begin{bmatrix}
1 & 1 &3  \\ 2 &2  &3  \\  1& 2 &2  \\\end{bmatrix}
$$

$$
\begin{cases}
x_{1}+2x_{2}+2x_{3}+x_{4}=0 \\
2x_{1}+x_{2}-2x_{3}-2x_{4}=0 \\
x_{1}-x_{2}-4x_{3}-3x_{4}=0 \\
\end{cases}
$$

# equation

$$
D(x) = \begin{cases}
\lim\limits_{x \to 0} \frac{a^x}{b+c}, & x<3 \\
\pi, & x=3 \\
\int_a^{3b}x_{ij}+e^2 \mathrm{d}x,& x>3 \\
\end{cases}
$$

$$
\begin{split}
\cos 2x &= \cos^2x - \sin^2x \\
&=2\cos^2x-1
\end{split}
$$
